feat: connect local palindrome profile

ReverseAddOverflowProfile.fst
@@ -2,6 +2,7 @@ module ReverseAddOverflowProfile
 
 open ReverseAdd
 open ReverseAddCarry
+open ReverseAddHighSum
 open FStar.List.Tot
 
 // Conversely, the overflow sum/carry relation reconstructs mirrored output
@@ -64,3 +65,126 @@ let reverse_trace_overflow_relation_implies_digit_symmetry
         10 * overflow_trace_carry_at xs (i + 1));
       assert (trace_digit_at xs i == trace_digit_at xs j);
       ()))
+
+let trace_local_palindrome_profile (xs:numeral 10) : prop =
+  (length (trace_digits xs) == length xs /\
+   nth (trace_carries xs) (length xs) == Some 0 /\
+   (forall i. i < length xs ==>
+     trace_sum_at xs i < 10)) \/
+  (length (trace_digits xs) == length xs + 1 /\
+   nth (trace_carries xs) (length xs) == Some 1 /\
+   (forall i. i <= length xs ==>
+     trace_sum_at xs i + overflow_trace_carry_at xs i +
+         10 * overflow_trace_carry_at xs (length xs - i + 1) ==
+       trace_sum_at xs (length xs - i) +
+         overflow_trace_carry_at xs (length xs - i) +
+         10 * overflow_trace_carry_at xs (i + 1)))
+
+let local_profile_196_is_false () : Lemma (
+    ~(trace_local_palindrome_profile digits_196)) =
+  assert (length (trace_digits digits_196) == length digits_196);
+  assert (nth (trace_carries digits_196) (length digits_196) == Some 0);
+  assert (trace_sum_at digits_196 1 == 18);
+  introduce (trace_local_palindrome_profile digits_196) ==> False
+  with (
+    eliminate
+      (length (trace_digits digits_196) == length digits_196 /\
+       nth (trace_carries digits_196) (length digits_196) == Some 0 /\
+       (forall i. i < length digits_196 ==>
+         trace_sum_at digits_196 i < 10)) \/
+      (length (trace_digits digits_196) == length digits_196 + 1 /\
+       nth (trace_carries digits_196) (length digits_196) == Some 1 /\
+       (forall i. i <= length digits_196 ==>
+         trace_sum_at digits_196 i + overflow_trace_carry_at digits_196 i +
+             10 * overflow_trace_carry_at digits_196
+               (length digits_196 - i + 1) ==
+           trace_sum_at digits_196 (length digits_196 - i) +
+             overflow_trace_carry_at digits_196 (length digits_196 - i) +
+             10 * overflow_trace_carry_at digits_196 (i + 1)))
+    with (
+      assert (trace_sum_at digits_196 1 < 10);
+      assert False)
+    and (
+      assert False))
+
+let trace_palindrome_implies_local_profile (xs:numeral 10)
+  : Lemma (requires (
+      xs <> [] /\ trace_digits xs == rev (trace_digits xs)))
+    (ensures (trace_local_palindrome_profile xs)) =
+  reverse_trace_palindrome_cases xs;
+  eliminate
+    (length (trace_digits xs) == length xs /\
+     nth (trace_carries xs) (length xs) == Some 0 /\
+     (forall i. i < length xs ==>
+       trace_carry_at xs i == trace_carry_at xs (length xs - 1 - i))) \/
+    (length (trace_digits xs) == length xs + 1 /\
+     nth (trace_carries xs) (length xs) == Some 1 /\
+     trace_digit_at xs 0 == 1)
+  with (
+    trace_no_overflow_palindrome_implies_sum_low xs;
+    assert (trace_local_palindrome_profile xs);
+    ())
+  and (
+    reverse_trace_overflow_sum_carry_relation xs;
+    assert (trace_local_palindrome_profile xs);
+    ())
+
+let trace_local_profile_implies_digit_symmetry (xs:numeral 10)
+  : Lemma (requires (
+      xs <> [] /\ trace_local_palindrome_profile xs))
+    (ensures (
+      (length (trace_digits xs) == length xs /\
+       (forall i. i < length xs ==>
+         trace_digit_at xs i ==
+           trace_digit_at xs (length xs - 1 - i))) \/
+      (length (trace_digits xs) == length xs + 1 /\
+       (forall i. i <= length xs ==>
+         trace_digit_at xs i ==
+           trace_digit_at xs (length xs - i))))) =
+  eliminate
+    (length (trace_digits xs) == length xs /\
+     nth (trace_carries xs) (length xs) == Some 0 /\
+     (forall i. i < length xs ==> trace_sum_at xs i < 10)) \/
+    (length (trace_digits xs) == length xs + 1 /\
+     nth (trace_carries xs) (length xs) == Some 1 /\
+     (forall i. i <= length xs ==>
+       trace_sum_at xs i + overflow_trace_carry_at xs i +
+           10 * overflow_trace_carry_at xs (length xs - i + 1) ==
+         trace_sum_at xs (length xs - i) +
+           overflow_trace_carry_at xs (length xs - i) +
+           10 * overflow_trace_carry_at xs (i + 1)))
+  with (
+    trace_no_overflow_low_sums_imply_digit_symmetry xs;
+    assert (length (trace_digits xs) == length xs /\
+      (forall i. i < length xs ==>
+        trace_digit_at xs i ==
+          trace_digit_at xs (length xs - 1 - i)));
+    ())
+  and (
+    reverse_trace_overflow_relation_implies_digit_symmetry xs;
+    assert (length (trace_digits xs) == length xs + 1 /\
+      (forall i. i <= length xs ==>
+        trace_digit_at xs i ==
+          trace_digit_at xs (length xs - i)));
+    ())
+
+let trace_local_profile_excludes_trace_palindrome
+  (xs:numeral 10) : Lemma (requires (
+      xs <> [] /\ ~(trace_local_palindrome_profile xs)))
+    (ensures (~ (palindrome #10 (trace_digits xs)))) =
+  introduce (palindrome #10 (trace_digits xs)) ==> False
+  with (
+    assert (trace_digits xs == rev (trace_digits xs));
+    trace_palindrome_implies_local_profile xs;
+    assert False)
+
+let reverse_add_local_profile_excludes_palindrome
+  (xs:numeral 10) : Lemma (requires (
+      canonical xs /\ xs <> [] /\
+      ~(trace_local_palindrome_profile xs)))
+    (ensures (~ (palindrome #10 (reverse_add xs)))) =
+  trace_digits_equals_reverse_add xs;
+  introduce (palindrome #10 (reverse_add xs)) ==> False
+  with (
+    assert (palindrome #10 (trace_digits xs));
+    trace_local_profile_excludes_trace_palindrome xs)
