Makefile
@@ -16,10 +16,10 @@ CHECK = "$(FSTAR)" \
 verify:
 	$(CHECK) ReverseAdd.fst
 	$(CHECK) ReverseAddCarry.fst
-	$(CHECK) ReverseAddOverflowProfile.fst
 	$(CHECK) ReverseAddCarrySummary.fst
 	$(CHECK) ReverseAddWitness.fst
 	$(CHECK) ReverseAddHighSum.fst
+	$(CHECK) ReverseAddOverflowProfile.fst
 	$(CHECK) ReverseAddBoundary.fst
 	$(CHECK) AbstractReachability.fst
 	$(CHECK) ReverseAddResidue.fst
